isabelle/CodeExport.thy
@@ -1,25 +1,42 @@
 theory CodeExport
-  imports BabParser BabLexer BabLoader "HOL-Library.Code_Binary_Nat"
+  imports FrontEnd "HOL-Library.Code_Binary_Nat"
 
 begin
 
 (* Code Export *)
 
-datatype CompileResult = CR_Success | CR_LexError | CR_ParseError
+datatype CompileResult = 
+  CR_Success          (* Successful compilation *)
+  | CR_LexError       (* Lexical error OR loader problem (module not found, etc.) *)
+  | CR_ParseError     (* Parse error *)
+  | CR_RenameError    (* Renamer error *)
 
+(* Function to convert front-end errors to a compile result *)
+fun frontend_errors_to_result :: "FrontEndError list \<Rightarrow> CompileResult" where
+  "frontend_errors_to_result [] = CR_LexError"
+| "frontend_errors_to_result (FrontEndError_Loader x # _) =
+  (case x of
+    LoaderError_ParseError _ \<Rightarrow> CR_ParseError
+    | LoaderError_PostParseError _ _ \<Rightarrow> CR_ParseError
+    | _ \<Rightarrow> CR_LexError
+  )"
+| "frontend_errors_to_result (FrontEndError_Renamer _ # _) = CR_RenameError"
+
+
+(* Main compiler entry point for testing *)
 fun run_compiler :: "string \<Rightarrow> CompileResult"
   where
 "run_compiler str =
-  (case lex ''Main'' str of
-    LR_Success tokens \<Rightarrow> 
-      (case run_parser parse_module ''stdin'' tokens of
-        PR_Success m _ _ \<Rightarrow>
-          (case post_parse_module m of
-            [] \<Rightarrow> CR_Success
-            | _ \<Rightarrow> CR_ParseError)
-      | PR_Error _ \<Rightarrow> CR_ParseError)
-  | LR_Error _ \<Rightarrow> CR_LexError)"
+  (let rawPkg = \<lparr> RP_Name = ''main'',
+                  RP_Dependencies = [],
+                  RP_ExportedModules = [],
+                  RP_Modules = [(''Main'', str)] \<rparr>;
+       result = compiler_front_end [rawPkg] ''main'' ''Main''
+   in case result of
+        Inr _ \<Rightarrow> CR_Success
+        | Inl errs \<Rightarrow> frontend_errors_to_result errs)"
 
-export_code run_compiler CR_Success CR_LexError CR_ParseError load_packages in Haskell
+export_code run_compiler CR_Success CR_LexError CR_ParseError CR_RenameError
+  in Haskell
 
 end
