isabelle/FrontEnd.thy
@@ -1,0 +1,100 @@
+theory FrontEnd
+  imports Main BabLoader BabRenamer
+begin
+
+(* Combined error type for the front end *)
+datatype FrontEndError =
+  FrontEndError_Loader LoaderError
+  | FrontEndError_Renamer RenameError
+
+(* Helper function to sequence a list of sum types where errors are lists *)
+(* If all are Inr, return Inr with list of successes *)
+(* If any are Inl, return Inl with concatenated list of all errors *)
+fun sequence_sum :: "('a list, 'b) sum list \<Rightarrow> ('a list, 'b list) sum"
+  where
+"sequence_sum [] = Inr []"
+| "sequence_sum (x # xs) =
+    (case sequence_sum xs of
+      Inl errs \<Rightarrow>
+        (case x of
+          Inl err \<Rightarrow> Inl (err @ errs)
+          | Inr _ \<Rightarrow> Inl errs)
+      | Inr results \<Rightarrow>
+        (case x of
+          Inl err \<Rightarrow> Inl err
+          | Inr result \<Rightarrow> Inr (result # results)))"
+
+(* Correctness property: if all inputs are successes, sequence_sum returns all the values *)
+lemma sequence_sum_all_success:
+  assumes "\<forall>x \<in> set xs. \<exists>v. x = Inr v"
+  shows "\<exists>vs. sequence_sum xs = Inr vs \<and> map Inr vs = xs"
+  using assms
+proof (induction xs)
+  case Nil
+  then show ?case by simp
+next
+  case (Cons x xs)
+  then obtain v where x_def: "x = Inr v"
+    by auto
+  from Cons.prems have "\<forall>x \<in> set xs. \<exists>v. x = Inr v"
+    by simp
+  then obtain vs where ih: "sequence_sum xs = Inr vs" "map Inr vs = xs"
+    using Cons.IH by blast
+  from x_def ih have "sequence_sum (x # xs) = Inr (v # vs)"
+    by simp
+  moreover have "map Inr (v # vs) = x # xs"
+    using x_def ih(2) by simp
+  ultimately show ?case
+    by simp
+qed
+
+(* Correctness property: if any input is an error, the output is an error *)
+lemma sequence_sum_preserves_errors:
+  assumes "\<exists>x \<in> set xs. (\<exists>errs. x = Inl errs)"
+  shows "\<exists>errs. sequence_sum xs = Inl errs"
+  using assms
+proof (induction xs)
+  case Nil
+  then show ?case by simp
+next
+  case (Cons x xs)
+  show ?case
+  proof (cases "\<exists>errs. x = Inl errs")
+    case True
+    then obtain errs where x_def: "x = Inl errs"
+      by blast
+    show ?thesis
+    proof (cases "sequence_sum xs")
+      case (Inl errs')
+      then show ?thesis
+        using x_def by simp
+    next
+      case (Inr vs)
+      then show ?thesis
+        using x_def by simp
+    qed
+  next
+    case False
+    then have "\<exists>x \<in> set xs. (\<exists>errs. x = Inl errs)"
+      using Cons.prems by auto
+    then obtain errs where "sequence_sum xs = Inl errs"
+      using Cons.IH by blast
+    then show ?thesis
+      by (cases x; simp)
+  qed
+qed
+
+(* Main front-end function *)
+fun compiler_front_end :: "RawPackage list \<Rightarrow> string \<Rightarrow> string \<Rightarrow>
+                           (FrontEndError list, BabModule list) sum"
+  where
+"compiler_front_end rawPkgs rootPkgName rootModName =
+  (case load_packages rawPkgs rootPkgName rootModName of
+    Inl loaderErrs \<Rightarrow> Inl (map FrontEndError_Loader loaderErrs)
+    | Inr loadedModules \<Rightarrow>
+      (let renameResults = map (\<lambda>module. rename_module module loadedModules) loadedModules
+       in case sequence_sum renameResults of
+            Inl renameErrs \<Rightarrow> Inl (map FrontEndError_Renamer renameErrs)
+            | Inr renamedModules \<Rightarrow> Inr renamedModules))"
+
+end
